![\Large x=\frac{-b\pm\sqrt{b^2-4ac}}{2a}](https://latex.codecogs.com/svg.latex?\Large&space;x=\frac{-b\pm\sqrt{b^2-4ac}}{2a}) 

Challenge: 

$\Large x=\frac{-b\pm\sqrt{b^2-4ac}}{2a}$

$$
\sqrt[3]{\frac{343^{6}+49^{15}}{343^{8}+49^{6}}} \\
= \sqrt[3]{\frac{(7^{3})^{6}+(7^{2})^{15}}{(7^{3})^{8}+(7^{2})^{6}}} \\
= \sqrt[3]{\frac{7^{18}+7^{30}}{7^{24}+7^{12}}} \\
= \sqrt[3]{\frac{{7^{18}}\times(1+7^{12})}{{7^{12}\times(1+7^{12})}}} \\
= \sqrt[3]{\frac{{7^{18}}\times\cancel{(1+7^{12})}}{{7^{12}\times\cancel{(1+7^{12})}}}} \\
= \sqrt[3]{7^{(18-12)}} = \sqrt[3]{7^6} \\
= 7^{(6/3)} = 7^2 = 49
$$